extraction: WIP on extracting embeddings for inductives

src/extraction/FStar.Extraction.ML.RegEmb.fst
@@ -27,19 +27,99 @@ open FStar.Extraction.ML.Syntax
 open FStar.Extraction.ML.UEnv
 open FStar.Syntax.Syntax
 
-module Print = FStar.Syntax.Print
 module BU    = FStar.Compiler.Util
-module SS    = FStar.Syntax.Subst
-module U     = FStar.Syntax.Util
-module PC    = FStar.Parser.Const
+module Code  = FStar.Extraction.ML.Code
 module EMB   = FStar.Syntax.Embeddings
+module PC    = FStar.Parser.Const
+module Print = FStar.Syntax.Print
+module S     = FStar.Syntax.Syntax
+module SS    = FStar.Syntax.Subst
+module Term  = FStar.Extraction.ML.Term
+module U     = FStar.Syntax.Util
 module Util  = FStar.Extraction.ML.Util
 
-let do_handle_plugin (g: uenv) (arity_opt: option int) (se: sigelt) : list mlmodule1 =
+exception Unsupported of string
+
+let mk e = with_ty MLTY_Top e
+let ml_none : mlexpr = mk (MLE_Name (["FStar"; "Pervasives"; "Native"], "None"))
+let ml_some : mlexpr = mk (MLE_Name (["FStar"; "Pervasives"; "Native"], "Some"))
+
+let tm_fvar_lid    = Ident.lid_of_str "FStar.Syntax.Syntax.Tm_fvar"
+let fv_eq_lid_lid  = Ident.lid_of_str "FStar.Syntax.Syntax.fv_eq_lid"
+let s_fvar_lid     = Ident.lid_of_str "FStar.Syntax.Syntax.fvar"
+let lid_of_str_lid = Ident.lid_of_str "Ident.lid_of_str" // :^)
+
+let fresh : string -> string =
+  let r = BU.mk_ref 0 in
+  fun s ->
+    let v = !r in
+    r := v+1;
+    s^"_"^(string_of_int v)
+
+let splitlast s = let x::xs = List.rev s in (List.rev xs, x)
+
+let mk_unembed (ctors: list sigelt) : mlexpr =
+  let e_branches : ref (list mlbranch) = BU.mk_ref [] in
+  let arg_v = fresh "tm" in
+  ctors |> List.iter (fun ctor ->
+    match ctor.sigel with
+    | Sig_datacon {lid; us; t; ty_lid; num_ty_params; mutuals} ->
+      let fv = fresh "fv" in
+      let bs, c = U.arrow_formals t in
+      (* let vs = List.map (fun b -> fresh (Ident.string_of_id b.binder_bv.ppname)) bs in *)
+
+      let pat_s = MLP_Const (MLC_String (Ident.string_of_lid lid)) in
+      let pat_args = MLP_CTor ((["Prims"], "Nil"), []) in
+      let pat_both = MLP_Tuple [pat_s; pat_args] in
+
+      let ret = mk (MLE_Name (splitlast (Ident.path_of_lid lid))) in
+      let ret = mk (MLE_App (ml_some, [ret])) in
+      let br = (pat_both, None, ret) in
+
+      e_branches := br :: !e_branches
+    | _ -> failwith "impossible, filter above"
+  );
+  let nomatch : mlbranch = (MLP_Wild, None, ml_none) in
+  let branches = List.rev (nomatch :: !e_branches) in
+  let sc = mk (MLE_Var arg_v) in
+  let def = mk (MLE_Match (sc, branches)) in
+  let lam = mk (MLE_Fun ([arg_v, MLTY_Top], def)) in
+  lam
+
+let mk_embed (ctors: list sigelt) : mlexpr =
+  let e_branches : ref (list mlbranch) = BU.mk_ref [] in
+  let arg_v = fresh "tm" in
+  ctors |> List.iter (fun ctor ->
+    match ctor.sigel with
+    | Sig_datacon {lid; us; t; ty_lid; num_ty_params; mutuals} ->
+      let fv = fresh "fv" in
+      let bs, c = U.arrow_formals t in
+      (* let vs = List.map (fun b -> fresh (Ident.string_of_id b.binder_bv.ppname)) bs in *)
+
+      let pat = MLP_CTor (splitlast (Ident.path_of_lid lid), []) in
+      let fvar = mk (MLE_Name (splitlast (Ident.path_of_lid s_fvar_lid))) in
+      let lid_of_str = mk (MLE_Name (splitlast (Ident.path_of_lid lid_of_str_lid))) in
+      let ret = mk (MLE_App (fvar, [
+                    mk (MLE_App (lid_of_str, [mk (MLE_Const (MLC_String (Ident.string_of_lid lid)))]));
+                    ml_none]))
+      in
+      let br = (pat, None, ret) in
+
+      e_branches := br :: !e_branches
+    | _ -> failwith "impossible, filter above"
+  );
+  let branches = List.rev !e_branches in
+  let sc = mk (MLE_Var arg_v) in
+  let def = mk (MLE_Match (sc, branches)) in
+  let lam = mk (MLE_Fun ([arg_v, MLTY_Top], def)) in
+  lam
+
+let __do_handle_plugin (g: uenv) (arity_opt: option int) (se: sigelt) : list mlmodule1 =
   // BU.print2 "Got plugin with attrs = %s; arity_opt=%s"
   //          (List.map Print.term_to_string se.sigattrs |> String.concat " ")
   //          (match arity_opt with None -> "None" | Some x -> "Some " ^ string_of_int x);
   let w = with_ty MLTY_Top in
+  let r = se.sigrng in
   match se.sigel with
   | Sig_let {lbs} ->
       let mk_registration lb : list mlmodule1 =
@@ -61,7 +141,45 @@ let do_handle_plugin (g: uenv) (arity_opt: option int) (se: sigelt) : list mlmod
          | None -> []
       in
       List.collect mk_registration (snd lbs)
+
+  | Sig_bundle {ses} ->
+    let typ_sigelt =
+      match List.filter (fun se -> match se.sigel with | Sig_inductive_typ _ -> true | _ -> false) ses with
+      | [se] -> se
+      | _ -> raise (Unsupported "mutual inductives")
+    in
+    let Sig_inductive_typ {lid=tlid} = typ_sigelt.sigel in
+    let name = Ident.string_of_id (List.last (Ident.ids_of_lid tlid)) in
+
+    let ctors = List.filter (fun se -> match se.sigel with | Sig_datacon _ -> true | _ -> false) ses in
+    let ml_name = mk (MLE_Const (MLC_String (Ident.string_of_lid tlid))) in
+    let ml_unembed = mk_unembed ctors in
+    let ml_embed = mk_embed ctors in
+    let def = mk (MLE_App (mk (MLE_Name (["FStar"; "Syntax"; "Embeddings"; "Base"], "mk_extracted_embedding")), [
+                    ml_name;
+                    ml_unembed;
+                    ml_embed]))
+    in
+    let lb = {
+      mllb_name     = "e_" ^ name;
+      mllb_tysc     = None;
+      mllb_add_unit = false;
+      mllb_def      = def;
+      mllb_meta     = [];
+      print_typ     = false;
+    }
+    in
+    [MLM_Let (NonRec, [lb])]
+
   | _ -> []
+
+let do_handle_plugin (g: uenv) (arity_opt: option int) (se: sigelt) : list mlmodule1 =
+  try __do_handle_plugin g arity_opt se with
+  | Unsupported msg ->
+    // FIXME: Change error code
+    Errors.log_issue se.sigrng (Errors.Warning_PluginNotImplemented,
+        BU.format2 "Could not generate a plugin for %s, reason = %s" (Print.sigelt_to_string_short se) msg);
+    []
 
 (* When extracting a plugin, each top-level definition marked with a `@plugin` attribute
    is extracted along with an invocation to FStar.Tactics.Native.register_tactic or register_plugin,
@@ -83,5 +201,9 @@ let maybe_register_plugin (g:uenv) (se:sigelt) : list mlmodule1 =
     else
       match plugin_with_arity se.sigattrs with
       | None -> []
+      (* ignore projectors and discriminators, they get a @@plugin attribute inherited
+      from the type, but we don't need to handle them. *)
+      | Some _ when List.existsb (function Projector _ | Discriminator _ -> true | _ -> false) se.sigquals ->
+        []
       | Some arity_opt ->
         do_handle_plugin g arity_opt se
